

# Structural Operational Semantics of Programs

Giuseppe De Giacomo

# Programs

We will consider a very simple programming language that we call “**while**”.

## while-programs

$a$	atomic action
$skip$	empty action
$\delta_1; \delta_2$	sequence
<b>if</b> $\phi$ <b>then</b> $\delta_1$ <b>else</b> $\delta_2$	if-then-else
<b>while</b> $\phi$ <b>do</b> $\delta$	while-loop

As atomic action we will typically consider assignments:

$$x := v$$

As test any boolean condition on the current state of the memory.

*Note that our considerations extend to full-fledged programming language (as Java).*

# Program semantics

Programs are syntactic objects.

*How do we assign a formal semantics to them?*

*Any idea of what the semantics should talk about?*

# Evaluation semantics

**Idea:** describe the overall result of the evaluation of the program.

## Evaluation semantics

Given a program  $\delta$  and a memory state  $s$  **compute the memory state  $s'$  obtained by executing  $\delta$  in  $s$ .**

More formally: define the **relation**:

$$(\delta, s) \longrightarrow s'$$

where  $\delta$  is a program,  $s$  is the memory state in which the program is evaluated, and  $s'$  is the memory state obtained by the evaluation.

Such a relation can be defined inductively in a standard way using the so called **evaluation (structural) rules**

# Evaluation semantics: references

The general approach we follow is the *structural operational semantics* approach [Plotkin81, Nielson&Nielson99].

This whole-computation semantics is often called: *evaluation semantics* or *natural semantics* or *computation semantic*.

# Evaluation rules for **while**-programs

## Evaluation rules for **while**-programs

$$\text{Act} : \frac{(a, s) \longrightarrow s'}{\text{true}} \quad \text{if } s \models \text{Pre}(a) \text{ and } s' = \text{Post}(a, s)$$

$$\text{special case: assignment} \quad \frac{(x := v, s) \longrightarrow s'}{\text{true}} \quad \text{if } s' = s[x = v]$$

$$\text{Skip} : \frac{(\text{skip}, s) \longrightarrow s}{\text{true}}$$

$$\text{Seq} : \frac{(\delta_1; \delta_2, s) \longrightarrow s'}{(\delta_1, s) \longrightarrow s'' \wedge (\delta_2, s'') \longrightarrow s'}$$

$$\text{if} : \frac{(\text{if } \phi \text{ then } \delta_1 \text{ else } \delta_2, s) \longrightarrow s'}{(\delta_1, s) \longrightarrow s'} \quad \text{if } s \models \phi \quad \frac{(\text{if } \phi \text{ then } \delta_1 \text{ else } \delta_2, s) \longrightarrow s'}{(\delta_2, s) \longrightarrow s'} \quad \text{if } s \models \neg \phi$$

$$\text{while} : \frac{(\text{while } \phi \text{ do } \delta, s) \longrightarrow s}{\text{true}} \quad \text{if } s \models \neg \phi \quad \frac{(\text{while } \phi \text{ do } \delta, s) \longrightarrow s'}{(\delta, s) \longrightarrow s'' \wedge (\text{while } \phi \text{ do } \delta, s'') \longrightarrow s'} \quad \text{if } s \models \phi$$

# Structural rules

The structural rules have the following schema:

$$\frac{\text{CONSEQUENT}}{\text{ANTECEDENT}} \text{ if SIDE-CONDITION}$$

which is to be interpreted logically as:

$$\forall (\text{ANTECEDENT} \wedge \text{SIDE-CONDITION} \supset \text{CONSEQUENT})$$

where  $\forall Q$  stands for the universal closure of all free variables occurring in  $Q$ , and, typically, ANTECEDENT, SIDE-CONDITION and CONSEQUENT share free variables.

The structural rules define inductively a relation, namely: **the smallest relation satisfying the rules.**

# Examples

## Example (evaluation semantics)

Compute  $s_f$  in the following cases, assuming that in the memory state  $S_0$  we have  $x = 10$  and  $y = 0$ :

- $(x := x + 1; x := x * 2, S_0) \longrightarrow s_f$
- $(x := x + 1;$   
    **if**  $(x < 10)$  **then**  $x := 0$  **else**  $x := 1$ ;  
     $x := x + 1, S_0) \longrightarrow s_f$
- $(y := 0; \textbf{while } (y < 4) \textbf{ do } \{x := x * 2; y := y + 1\}, S_0) \longrightarrow s_f$



a)

$$(x := x + 1; x := x * 2, S_0) \longrightarrow s_f$$

$$S_0: \begin{cases} x = 10 \\ y = 0 \end{cases}$$

$$\text{Seq: } \frac{(\delta_1; \delta_2, s) \longrightarrow s'}{(\delta_1, s) \longrightarrow s'' \wedge (\delta_2, s'') \longrightarrow s'}$$

$$\frac{(x := x + 1; x := x \cdot 2, S_0) \rightarrow S_F}{(x := x + 1, S_0) \rightarrow S' \wedge (x := x \cdot 2, S') \rightarrow S_F}$$

$$\frac{(x := x + 1; x := x \cdot 2, S_0) \rightarrow S_F}{(x := x + 1, S_0) \rightarrow S_1 \wedge (x := x \cdot 2, S_1) \rightarrow S_F}$$

TRUE                      TRUE

$$S_1: \begin{cases} x = 11 \\ y = 0 \end{cases} \quad S_F: \begin{cases} x = 22 \\ y = 0 \end{cases}$$

b)

$$(x := x + 1; \text{if } (x < 10) \text{ then } x := 0 \text{ else } x := 1; x := x + 1, S_0) \longrightarrow s_f$$

$$S_0: \begin{cases} x = 10 \\ y = 0 \end{cases}$$

$$\text{if: } \frac{(\text{if } \phi \text{ then } \delta_1 \text{ else } \delta_2, s) \longrightarrow s'}{(\delta_1, s) \longrightarrow s'} \quad \text{if } s \models \phi \quad \frac{(\text{if } \phi \text{ then } \delta_1 \text{ else } \delta_2, s) \longrightarrow s'}{(\delta_2, s) \longrightarrow s'} \quad \text{if } s \models \neg \phi$$

$$\frac{x := x + 1; \text{IF } (x < 10) \text{ THEN } x := 0 \text{ ELSE } x := 1; x := x + 1, S_0 \rightarrow S_F}{(x := x + 1, S_0) \rightarrow S_1 \wedge (\text{IF } (x < 10) \text{ THEN } x := 0 \text{ ELSE } x := 1; x := x + 1, S_1) \rightarrow S_F}$$

TRUE

$$\frac{(\text{IF } (x < 10) \text{ THEN } x := 0 \text{ ELSE } x := 1, S_1) \rightarrow S_2 \wedge (x := x + 1, S_2) \rightarrow S_F}{(x := 1, S_1) \rightarrow S_2}$$

TRUE

$$S_1: \begin{cases} x = 11 \\ y = 0 \end{cases} \quad S_2: \begin{cases} x = 1 \\ y = 0 \end{cases} \quad S_F: \begin{cases} x = 2 \\ y = 0 \end{cases}$$

c)

$$(\text{while } (y < 1) \text{ do } \{x := x * 2; y := y + 1\}, S_0) \longrightarrow s_f$$

$$S_0: \begin{cases} x = 10 \\ y = 0 \end{cases}$$

$$\text{while: } \frac{(\text{while } \phi \text{ do } \delta, s) \longrightarrow s}{\text{true}} \quad \text{if } s \models \neg \phi \quad \frac{(\text{while } \phi \text{ do } \delta, s) \longrightarrow s'}{(\delta, s) \longrightarrow s'' \wedge (\text{while } \phi \text{ do } \delta, s'') \longrightarrow s'} \quad \text{if } s \models \phi$$

$$\frac{(\text{WHILE } (y < 1) \text{ DO } \{x := x \cdot 2; y := y + 1\}, S_0) \rightarrow S_F}{(x := x \cdot 2; y := y + 1, S_0) \rightarrow S_1 \wedge (\text{WHILE } (y < 1) \text{ DO } \{x := x \cdot 2; y := y + 1\}, S_1) \rightarrow S_F}$$

$$\frac{(x := x \cdot 2, S_0) \rightarrow S_1 \wedge (y := y + 1, S_1) \rightarrow S_2}{(x := x \cdot 2, S_1) \rightarrow S_3 \wedge (y := y + 1, S_3) \rightarrow S_F}$$

TRUE                      TRUE                      TRUE                      TRUE

$$S_1: \begin{cases} x = 20 \\ y = 0 \end{cases} \quad S_2: \begin{cases} x = 20 \\ y = 1 \end{cases} \quad S_3: \begin{cases} x = 40 \\ y = 0 \end{cases} \quad S_F: \begin{cases} x = 40 \\ y = 1 \end{cases}$$

# Transition semantics

**Idea:** describe the result of executing a **single step** of the program.

## Transition semantics

- Given a program  $\delta$  and a memory state  $s$  **compute the memory state  $s'$  and the program  $\delta'$  that remains to be executed obtained by executing a single step of  $\delta$  in  $s$ .**
- Assert when a program  $\delta$  can be considered **successfully terminated** in a memory state  $s$ .

# Transition semantics

More formally:

## Transition semantics

- Define the **relation** “*Trans*” denoted by “ $\longrightarrow$ ”:

$$(\delta, s) \longrightarrow (\delta', s')$$

where  $\delta$  is a program,  $s$  is the memory state in which the program is executed, and  $s'$  is the memory state obtained by executing a single step of  $\delta$  and  $\delta'$  is what remains to be executed of  $\delta$  after such a single step.

- Define a **predicate** “*Final*” and denoted by “ $\checkmark$ ”:

$$(\delta, s)^\checkmark$$

where  $\delta$  is a program that can be considered (successfully) terminated in the memory state  $s$ .

Such a relation and predicate can be defined inductively in a standard way, using the so called **transition (structural) rules**

# Transition semantics: references

The general approach we follow is the *structural operational semantics* approach [Plotkin81, Nielson&Nielson99].

This single-step semantics is often called: *transition semantics* or *computation semantics*.

# Transition rules for **while**-programs

## Transition rules for **while**-programs

$$Act : \frac{(a, s) \longrightarrow (\epsilon, s')}{true} \quad \text{if } s \models Pre(a) \text{ and } s' = Post(a, s)$$

$$\text{special case: assignment} \quad \frac{(x := v, s) \longrightarrow (\epsilon, s')}{true} \quad \text{if } s' = s[x = v]$$

$$Skip : \frac{(skip, s) \longrightarrow (\epsilon, s)}{true}$$

$$Seq : \frac{(\delta_1; \delta_2, s) \longrightarrow (\delta'_1; \delta_2, s')}{(\delta_1, s) \longrightarrow (\delta'_1, s')} \quad \frac{(\delta_1; \delta_2, s) \longrightarrow (\delta'_2, s')}{(\delta_2, s) \longrightarrow (\delta'_2, s')} \quad \text{if } (\delta_1, s) \checkmark$$

$$if : \frac{(\text{if } \phi \text{ then } \delta_1 \text{ else } \delta_2, s) \longrightarrow (\delta'_1, s')}{(\delta_1, s) \longrightarrow (\delta'_1, s')} \quad \text{if } s \models \phi \quad \frac{(\text{if } \phi \text{ then } \delta_1 \text{ else } \delta_2, s) \longrightarrow (\delta'_2, s')}{(\delta_2, s) \longrightarrow (\delta'_2, s')} \quad \text{if } s \models \neg \phi$$

$$while : \frac{(\text{while } \phi \text{ do } \delta, s) \longrightarrow (\delta', \text{while } \phi \text{ do } \delta, s')}{(\delta, s) \longrightarrow (\delta', s')} \quad \text{if } s \models \phi$$

$\epsilon$  is the empty program.

# Termination rules for **while**-programs

## Termination rules for **while**-programs

$$\epsilon : \frac{(\epsilon, s) \checkmark}{true}$$

$$Seq : \frac{(\delta_1; \delta_2, s) \checkmark}{(\delta_1, s) \checkmark \wedge (\delta_2; s) \checkmark}$$

$$if : \frac{(\text{if } \phi \text{ then } \delta_1 \text{ else } \delta_2, s) \checkmark}{(\delta_1, s) \checkmark} \quad \text{if } s \models \phi \qquad \frac{(\text{if } \phi \text{ then } \delta_1 \text{ else } \delta_2, s) \checkmark}{(\delta_2, s) \checkmark} \quad \text{if } s \models \neg \phi$$

$$while : \frac{(\text{while } \phi \text{ do } \delta, s) \checkmark}{true} \quad \text{if } s \models \neg \phi \qquad \frac{(\text{while } \phi \text{ do } \delta, s) \checkmark}{(\delta, s) \checkmark} \quad \text{if } s \models \phi$$

## Structural rules (as before)

The structural rules have the following schema:

$$\frac{\text{CONSEQUENT}}{\text{ANTECEDENT}} \text{ if SIDE-CONDITION}$$

which is to be interpreted logically as:

$$\forall (\text{ANTECEDENT} \wedge \text{SIDE-CONDITION} \supset \text{CONSEQUENT})$$

where  $\forall Q$  stands for the universal closure of all free variables occurring in  $Q$ , and, typically, ANTECEDENT, SIDE-CONDITION and CONSEQUENT share free variables.

The structural rules define inductively a relation, namely: **the smallest relation satisfying the rules.**

# Example

## Example (transition semantics)

Compute  $\delta', s'$  in the following cases, assuming that in the memory state  $S_0$  we have  $x = 10$  and  $y = 0$ :

- $(x := x + 1; x := x * 2, S_0) \longrightarrow (\delta', s')$
- $(x := x + 1;$   
    **if**  $(x < 10)$  **then**  $x := 0$  **else**  $x := 1$ ;  
     $x := x + 1, S_0) \longrightarrow (\delta', s')$
- $(y := 0; \textbf{while } (y < 4) \textbf{ do } \{x := x * 2; y := y + 1\}, S_0) \longrightarrow (\delta', s')$



# Evaluation vs. transition semantics

How do we characterize a whole computation using single steps?

First we define the relation, named  $Trans^*$ , denoted by  $\longrightarrow^*$  by the following rules:

Reflexive-transitive closure of single steps: “ $\longrightarrow^*$ ”

$$0 \text{ step : } \frac{(\delta, s) \longrightarrow^* (\delta, s)}{true}$$

$$n \text{ step : } \frac{(\delta, s) \longrightarrow^* (\delta'', s'')}{(\delta, s) \longrightarrow (\delta', s') \wedge (\delta', s') \longrightarrow^* (\delta'', s'')} \quad (\text{for some } \delta', s')$$

Notice that such relation is the **reflexive-transitive closure** of (single step)  $\longrightarrow$ .

Then it can be shown that:

## Theorem

For every **while-program**  $\delta$  and states  $s$  and  $s_f$ :

$$(\delta, s_0) \longrightarrow s_f \quad \equiv \quad (\delta, s_0) \longrightarrow^* (\delta_f, s_f) \wedge (\delta_f, s_f)^\vee \quad \text{for some } \delta_f$$

## Example

### Example (Computing evaluation through repeated transitions)

Compute  $s_f$ , using the definition based on  $\longrightarrow^*$ , in the following cases, assuming that in the memory state  $S_0$  we have  $x = 10$  and  $y = 0$ :

- $(x := x + 1; x := x * 2, S_0) \longrightarrow s_f$
- $(x := x + 1;$   
    **if**  $(x < 10)$  **then**  $x := 0$  **else**  $x := 1$ ;  
     $x := x + 1, S_0) \longrightarrow s_f$
- $(y := 0; \textbf{while } (y < 4) \textbf{ do } \{x := x * 2; y := y + 1\}, S_0) \longrightarrow s_f$

~~( $\delta, s$ )~~, while ( $y < 1$ ) do  $\{x := x * 2; y := y + 1\}, S_0) \longrightarrow (\delta', s')$

$$S_0 \begin{cases} x=10 \\ y=0 \end{cases}$$

$$\text{while} : \frac{(\text{while } \phi \text{ do } \delta, s) \longrightarrow (\delta'; \text{while } \phi \text{ do } \delta, s')}{(\delta, s) \longrightarrow (\delta', s')} \quad \text{if } s \models \phi$$

$$\underline{\text{WHILE } (y < 1) \text{ DO } \{x = x \cdot 2; y := y + 1\}, S_0) \rightarrow (\delta', s')}$$

$$\frac{(x = x \cdot 2, S_0 \rightarrow \delta_1, S_1)}{\text{TRUE}}$$

$$\begin{aligned} \delta' &= y := y + 1; \text{WHILE} \dots \\ \delta_1 &= \epsilon \end{aligned}$$

$$\underline{\text{WHILE } (y < 1) \text{ DO } \{x = x \cdot 2; y := y + 1\}, S_0) \rightarrow (y := y + 1; \text{WHILE} \dots, S_1)}$$

$$\frac{(x = x \cdot 2, S_0 \rightarrow \epsilon, S_1)}{\text{TRUE}}$$

$$S_1 \begin{cases} x=20 \\ y=0 \end{cases}$$

$$\underline{(y := y + 1; \text{WHILE} \dots, S_1) \rightarrow (\delta'', s'')}$$

$$\frac{(y := y + 1, S_1) \rightarrow (\delta_2, s'')}{\text{TRUE}}$$

$$\delta'' = \delta_2; \text{WHILE} \dots$$

$$\delta_2 = \epsilon$$

$$S_2 \begin{cases} x=20 \\ y=1 \end{cases}$$

$$\underline{(\epsilon; \text{WHILE } (y < 1) \text{ DO } \dots, S_2) \rightarrow (\delta''', s''')}$$

$$\underline{(\epsilon; \text{WHILE } (y < 1) \text{ DO } \dots, S_2)^\checkmark}$$

$$\frac{(\epsilon, S_2)^\checkmark \wedge (\text{WHILE } (y < 1) \text{ DO } \dots, S_2)^\checkmark}{\text{TRUE}} \quad \text{TRUE}$$

# Concurrency

The transition semantics extends immediately to constructs for concurrency: The evaluation semantics can still be defined but only in terms of the transition semantics (as above).

We model concurrent processes by **interleaving**: *A concurrent execution of two processes is one where the primitive actions in both processes occur, interleaved in some fashion.*

It is OK for a process to remain **blocked** for a while, the other processes will continue and eventually unblock it.

# Additional constructs for concurrency

## Constructs for concurrency

$(\delta_1 \parallel \delta_2)$	concurrent execution
<b>if</b> $\phi$ <b>then</b> $\delta_1$ <b>else</b> $\delta_2$	synchronized conditional
<b>while</b> $\phi$ <b>do</b> $\delta$	synchronized loop

For the latter, we observe that our transition rules for **if** and **while** enforce already synchronization': *testing the condition  $\phi$  does not involve a transition per se, the evaluation of the condition and the first action of the branch chosen are executed as an atomic unit.*

*Note: synchronized **if** and **while** are similar to test-and-set atomic instructions used to build semaphores in concurrent programming.*

# Additional transition and termination rules for concurrency

The construct  $\delta_1 \parallel \delta_2$  is genuinely new.

It represents concurrency by interleaving:

## Transition and termination rules for concurrency

$$\begin{array}{l} \text{transition :} \quad \frac{(\delta_1 \parallel \delta_2, s) \longrightarrow (\delta'_1 \parallel \delta_2, s')}{(\delta_1, s) \longrightarrow (\delta'_1, s')} \quad \frac{(\delta_1 \parallel \delta_2, s) \longrightarrow (\delta_1 \parallel \delta'_2, s')}{(\delta_2, s) \longrightarrow (\delta'_2, s')} \\ \\ \text{termination :} \quad \frac{(\delta_1 \parallel \delta_2, s) \checkmark}{(\delta_1, s) \checkmark \wedge (\delta_2, s) \checkmark} \end{array}$$

The presence of  $\delta_1 \parallel \delta_2$  makes the transition relation **nondeterministic** (NB: “devilish nondeterminism”).